src/tactics/ml/FStar_Tactics_Builtins.ml
@@ -66,8 +66,8 @@ let trivial: unit -> unit __tac = fun () -> __trivial
 let __norm (s: FStar_Reflection_Data.norm_step list): unit __tac = from_tac_1 B.norm s
 let norm: FStar_Reflection_Data.norm_step list -> unit -> unit __tac = fun s -> fun () -> __norm s
 
-let __intro (s_opt:string option): RT.binder __tac = from_tac_1 B.intro_named s_opt
-let intro: string option -> unit -> RT.binder __tac = fun s_opt -> fun () -> __intro s_opt
+let __intro_named (s_opt:string option): RT.binder __tac = from_tac_1 B.intro_named s_opt
+let intro_named: string option -> unit -> RT.binder __tac = fun s_opt -> fun () -> __intro_named s_opt
 
 let __revert: unit __tac = from_tac_0 B.revert
 let revert: unit -> unit __tac = fun () -> __revert
